merged `FSHValType` with `DSHType`
All `FSHValType` occurences were replaced with `DSHType`.
Constructors mapping:

FSHnatValType -> DSHnat
FSHFloatValType -> DSHCType
FSHVecValType -> DSHPtr

`DSHPtr` constructor was extended to keep track of
size of memory block (vector) it is pointing to.

In particular, this addresses a shortcoming that
size of global variables was lost during MSH->DSH
compilation.

To make it work we removed avility to pass memory blocks
by value in DHSCOL. This was not an intended feature of the
language anyway.

ml/testeval.ml
@@ -26,10 +26,11 @@ let output_ll_file filename ast =
   Out_channel.close channel
 
 let gsize t =
+  let open FSigmaHCOL.MDSHCOLOnFloat64 in
   match t with
-  | FSHnatValType -> 1
-  | FSHFloatValType -> 1
-  | FSHvecValType n -> int_of_Int64 n
+  | DSHnat -> 1
+  | DSHCType -> 1
+  | DSHPtr n -> int_of_Int64 n
 
 let string_of_FloatV fv =
   Float.to_string (camlfloat_of_coqfloat fv)
